broke the code when switching from Sort to Type... but got some of it working

src/free.lean
@@ -1,28 +1,38 @@
 import basic
 
+import data.seq
+import order.bounded_lattice
+
+open seq (map) (reduce) (all)
+open lattice
+
+
 section
 
-parameters (S : signature) (X : Sort*)
 
-inductive term
+inductive term  {S : signature} (X : Type) : Type
 | var : X → term
-| app (f) : (S.ρ f → term) → term
+| app : ∀ (f : S.F), (S.ρ f → term) → term
 
 open term
 
-def free : algebra S :=
-⟨term, app⟩
 
-parameters (A : algebra S) (h : X → A)
+def free {S : signature} (X : Type) : algebra S :=
+⟨@term S X, @term.app S X⟩
+
+#print free
+
+variable (S : signature) --(X : Type 0)
+variables (A : algebra S) (Y: Type) (g : Y → A.1)
 
 -- Free algebra is really free: existence & uniqueness
-
-def imap : free → A
-| (var .(S) x) := h x
-| (app f a)    := A f (imap ∘ a)
+def imap : (@free S Y) → A.1
+| (term.var x) := g x
+| (term.app f a) := (A f) (imap ∘ a)
+--(λ (i : S.ρ f), imap (a i))
 
 lemma imap_is_hom : homomorphic imap :=
-λ f a, by rw [show free f a = app f a, from rfl,
+λ f a, by rw [show @free S Y f a = app f a, from rfl,
               show imap (app f a) = A f (imap ∘ a), from rfl]
 
 lemma hom_unique : ∀ {α β : free → A},
@@ -34,3 +44,14 @@ lemma hom_unique : ∀ {α β : free → A},
 end
 
 end
+
+
+
+
+
+
+
+
+
+
+
