src/basic.lean
@@ -1,7 +1,8 @@
 import data.set2
 
 structure signature :=
-mk :: (F : Sort*) (ρ : F → Sort*)
+mk :: (F : Type) (ρ : F → Type)
+
 
 section
 parameter (S : signature)
@@ -11,14 +12,16 @@ def algebra_on (α) :=
 Π f, (S.ρ f → α) → α
 
 -- An algebra pairs a carrier with an interpretation
-def algebra :=
+def algebra := 
 psigma algebra_on
 
 instance alg_univ : has_coe_to_sort algebra :=
 ⟨_, psigma.fst⟩
 
-instance alg_ops : has_coe_to_fun algebra :=
+
+instance alg_ops : has_coe_to_fun algebra := 
 ⟨_, psigma.snd⟩
+
 
 end
 
